feat: Adding a storage option to the KeyStore (#594)
The key store now allows for both a default DynamoDB table,
or any custom storage system.

The important aspect about the key store
is the fact that branch keys can be versioned easily,
and are cryptographically safe to use.
The actual storage medium is not important.

See: https://github.com/awslabs/aws-encryption-sdk-specification/blob/master/changes/2024-6-17_key-store-persistance/background.md#background

AwsCryptographicMaterialProviders/runtimes/python/src/aws_cryptographic_material_providers/smithygenerated/aws_cryptography_keystore/dafny_to_smithy.py
@@ -3,13 +3,195 @@
 # Do not modify this file. This file is machine generated, and any changes to it will be overwritten.
 
 from aws_cryptographic_material_providers.internaldafny.generated.AwsCryptographyKeyStoreTypes import (
+    HierarchicalKeyType_ActiveHierarchicalSymmetricBeacon,
+    HierarchicalKeyType_ActiveHierarchicalSymmetricVersion,
+    HierarchicalKeyType_HierarchicalSymmetricVersion,
     KMSConfiguration_discovery,
     KMSConfiguration_kmsKeyArn,
     KMSConfiguration_kmsMRKeyArn,
     KMSConfiguration_mrDiscovery,
+    KeyManagement_kms,
+    Storage_custom,
+    Storage_ddb,
 )
 import aws_cryptographic_material_providers.smithygenerated.aws_cryptography_keystore.dafny_to_smithy
 import aws_cryptographic_material_providers.smithygenerated.aws_cryptography_keystore.models
+
+
+def aws_cryptography_keystore_EncryptedHierarchicalKey(dafny_input):
+    return aws_cryptographic_material_providers.smithygenerated.aws_cryptography_keystore.models.EncryptedHierarchicalKey(
+        identifier=b"".join(
+            ord(c).to_bytes(2, "big") for c in dafny_input.Identifier
+        ).decode("utf-16-be"),
+        type=aws_cryptographic_material_providers.smithygenerated.aws_cryptography_keystore.dafny_to_smithy.aws_cryptography_keystore_HierarchicalKeyType(
+            dafny_input.Type
+        ),
+        create_time=b"".join(
+            ord(c).to_bytes(2, "big") for c in dafny_input.CreateTime
+        ).decode("utf-16-be"),
+        kms_arn=b"".join(ord(c).to_bytes(2, "big") for c in dafny_input.KmsArn).decode(
+            "utf-16-be"
+        ),
+        encryption_context={
+            b"".join(ord(c).to_bytes(2, "big") for c in key)
+            .decode("utf-16-be"): b"".join(ord(c).to_bytes(2, "big") for c in value)
+            .decode("utf-16-be")
+            for (key, value) in dafny_input.EncryptionContext.items
+        },
+        ciphertext_blob=bytes(dafny_input.CiphertextBlob),
+    )
+
+
+def aws_cryptography_keystore_HierarchicalKeyType(dafny_input):
+    # Convert HierarchicalKeyType
+    if isinstance(dafny_input, HierarchicalKeyType_ActiveHierarchicalSymmetricVersion):
+        HierarchicalKeyType_union_value = aws_cryptographic_material_providers.smithygenerated.aws_cryptography_keystore.models.HierarchicalKeyTypeActiveHierarchicalSymmetricVersion(
+            aws_cryptographic_material_providers.smithygenerated.aws_cryptography_keystore.dafny_to_smithy.aws_cryptography_keystore_ActiveHierarchicalSymmetric(
+                dafny_input.ActiveHierarchicalSymmetricVersion
+            )
+        )
+    elif isinstance(dafny_input, HierarchicalKeyType_HierarchicalSymmetricVersion):
+        HierarchicalKeyType_union_value = aws_cryptographic_material_providers.smithygenerated.aws_cryptography_keystore.models.HierarchicalKeyTypeHierarchicalSymmetricVersion(
+            aws_cryptographic_material_providers.smithygenerated.aws_cryptography_keystore.dafny_to_smithy.aws_cryptography_keystore_HierarchicalSymmetric(
+                dafny_input.HierarchicalSymmetricVersion
+            )
+        )
+    elif isinstance(dafny_input, HierarchicalKeyType_ActiveHierarchicalSymmetricBeacon):
+        HierarchicalKeyType_union_value = aws_cryptographic_material_providers.smithygenerated.aws_cryptography_keystore.models.HierarchicalKeyTypeActiveHierarchicalSymmetricBeacon(
+            aws_cryptographic_material_providers.smithygenerated.aws_cryptography_keystore.dafny_to_smithy.aws_cryptography_keystore_ActiveHierarchicalSymmetricBeacon(
+                dafny_input.ActiveHierarchicalSymmetricBeacon
+            )
+        )
+    else:
+        raise ValueError("No recognized union value in union type: " + str(dafny_input))
+
+    return HierarchicalKeyType_union_value
+
+
+def aws_cryptography_keystore_ActiveHierarchicalSymmetric(dafny_input):
+    return aws_cryptographic_material_providers.smithygenerated.aws_cryptography_keystore.models.ActiveHierarchicalSymmetric(
+        version=b"".join(ord(c).to_bytes(2, "big") for c in dafny_input.Version).decode(
+            "utf-16-be"
+        ),
+    )
+
+
+def aws_cryptography_keystore_HierarchicalSymmetric(dafny_input):
+    return aws_cryptographic_material_providers.smithygenerated.aws_cryptography_keystore.models.HierarchicalSymmetric(
+        version=b"".join(ord(c).to_bytes(2, "big") for c in dafny_input.Version).decode(
+            "utf-16-be"
+        ),
+    )
+
+
+def aws_cryptography_keystore_ActiveHierarchicalSymmetricBeacon(dafny_input):
+    return (
+        aws_cryptographic_material_providers.smithygenerated.aws_cryptography_keystore.models.ActiveHierarchicalSymmetricBeacon()
+    )
+
+
+def aws_cryptography_keystore_WriteNewEncryptedBranchKeyInput(dafny_input):
+    return aws_cryptographic_material_providers.smithygenerated.aws_cryptography_keystore.models.WriteNewEncryptedBranchKeyInput(
+        active=aws_cryptographic_material_providers.smithygenerated.aws_cryptography_keystore.dafny_to_smithy.aws_cryptography_keystore_EncryptedHierarchicalKey(
+            dafny_input.Active
+        ),
+        version=aws_cryptographic_material_providers.smithygenerated.aws_cryptography_keystore.dafny_to_smithy.aws_cryptography_keystore_EncryptedHierarchicalKey(
+            dafny_input.Version
+        ),
+        beacon=aws_cryptographic_material_providers.smithygenerated.aws_cryptography_keystore.dafny_to_smithy.aws_cryptography_keystore_EncryptedHierarchicalKey(
+            dafny_input.Beacon
+        ),
+    )
+
+
+def aws_cryptography_keystore_WriteNewEncryptedBranchKeyOutput(dafny_input):
+    return (
+        aws_cryptographic_material_providers.smithygenerated.aws_cryptography_keystore.models.WriteNewEncryptedBranchKeyOutput()
+    )
+
+
+def aws_cryptography_keystore_WriteNewEncryptedBranchKeyVersionInput(dafny_input):
+    return aws_cryptographic_material_providers.smithygenerated.aws_cryptography_keystore.models.WriteNewEncryptedBranchKeyVersionInput(
+        active=aws_cryptographic_material_providers.smithygenerated.aws_cryptography_keystore.dafny_to_smithy.aws_cryptography_keystore_EncryptedHierarchicalKey(
+            dafny_input.Active
+        ),
+        version=aws_cryptographic_material_providers.smithygenerated.aws_cryptography_keystore.dafny_to_smithy.aws_cryptography_keystore_EncryptedHierarchicalKey(
+            dafny_input.Version
+        ),
+        old_active=aws_cryptographic_material_providers.smithygenerated.aws_cryptography_keystore.dafny_to_smithy.aws_cryptography_keystore_EncryptedHierarchicalKey(
+            dafny_input.oldActive
+        ),
+    )
+
+
+def aws_cryptography_keystore_WriteNewEncryptedBranchKeyVersionOutput(dafny_input):
+    return (
+        aws_cryptographic_material_providers.smithygenerated.aws_cryptography_keystore.models.WriteNewEncryptedBranchKeyVersionOutput()
+    )
+
+
+def aws_cryptography_keystore_GetEncryptedActiveBranchKeyInput(dafny_input):
+    return aws_cryptographic_material_providers.smithygenerated.aws_cryptography_keystore.models.GetEncryptedActiveBranchKeyInput(
+        identifier=b"".join(
+            ord(c).to_bytes(2, "big") for c in dafny_input.Identifier
+        ).decode("utf-16-be"),
+    )
+
+
+def aws_cryptography_keystore_GetEncryptedActiveBranchKeyOutput(dafny_input):
+    return aws_cryptographic_material_providers.smithygenerated.aws_cryptography_keystore.models.GetEncryptedActiveBranchKeyOutput(
+        item=aws_cryptographic_material_providers.smithygenerated.aws_cryptography_keystore.dafny_to_smithy.aws_cryptography_keystore_EncryptedHierarchicalKey(
+            dafny_input.Item
+        ),
+    )
+
+
+def aws_cryptography_keystore_GetEncryptedBranchKeyVersionInput(dafny_input):
+    return aws_cryptographic_material_providers.smithygenerated.aws_cryptography_keystore.models.GetEncryptedBranchKeyVersionInput(
+        identifier=b"".join(
+            ord(c).to_bytes(2, "big") for c in dafny_input.Identifier
+        ).decode("utf-16-be"),
+        version=b"".join(ord(c).to_bytes(2, "big") for c in dafny_input.Version).decode(
+            "utf-16-be"
+        ),
+    )
+
+
+def aws_cryptography_keystore_GetEncryptedBranchKeyVersionOutput(dafny_input):
+    return aws_cryptographic_material_providers.smithygenerated.aws_cryptography_keystore.models.GetEncryptedBranchKeyVersionOutput(
+        item=aws_cryptographic_material_providers.smithygenerated.aws_cryptography_keystore.dafny_to_smithy.aws_cryptography_keystore_EncryptedHierarchicalKey(
+            dafny_input.Item
+        ),
+    )
+
+
+def aws_cryptography_keystore_GetEncryptedBeaconKeyInput(dafny_input):
+    return aws_cryptographic_material_providers.smithygenerated.aws_cryptography_keystore.models.GetEncryptedBeaconKeyInput(
+        identifier=b"".join(
+            ord(c).to_bytes(2, "big") for c in dafny_input.Identifier
+        ).decode("utf-16-be"),
+    )
+
+
+def aws_cryptography_keystore_GetEncryptedBeaconKeyOutput(dafny_input):
+    return aws_cryptographic_material_providers.smithygenerated.aws_cryptography_keystore.models.GetEncryptedBeaconKeyOutput(
+        item=aws_cryptographic_material_providers.smithygenerated.aws_cryptography_keystore.dafny_to_smithy.aws_cryptography_keystore_EncryptedHierarchicalKey(
+            dafny_input.Item
+        ),
+    )
+
+
+def aws_cryptography_keystore_GetKeyStorageInfoInput(dafny_input):
+    return (
+        aws_cryptographic_material_providers.smithygenerated.aws_cryptography_keystore.models.GetKeyStorageInfoInput()
+    )
+
+
+def aws_cryptography_keystore_GetKeyStorageInfoOutput(dafny_input):
+    return aws_cryptographic_material_providers.smithygenerated.aws_cryptography_keystore.models.GetKeyStorageInfoOutput(
+        name=bytes(dafny_input.Name.Elements).decode("utf-8"),
+        logical_name=bytes(dafny_input.LogicalName.Elements).decode("utf-8"),
+    )
 
 
 def smithy_api_Unit():
@@ -244,11 +426,100 @@ def aws_cryptography_keystore_GetBeaconKeyOutput(dafny_input):
     )
 
 
-def aws_cryptography_keystore_DdbClientReference(dafny_input):
-    return dafny_input._impl
+def aws_cryptography_keystore_KeyManagement(dafny_input):
+    # Convert KeyManagement
+    if isinstance(dafny_input, KeyManagement_kms):
+        KeyManagement_union_value = aws_cryptographic_material_providers.smithygenerated.aws_cryptography_keystore.models.KeyManagementKms(
+            aws_cryptographic_material_providers.smithygenerated.aws_cryptography_keystore.dafny_to_smithy.aws_cryptography_keystore_AwsKms(
+                dafny_input.kms
+            )
+        )
+    else:
+        raise ValueError("No recognized union value in union type: " + str(dafny_input))
+
+    return KeyManagement_union_value
+
+
+def aws_cryptography_keystore_AwsKms(dafny_input):
+    return aws_cryptographic_material_providers.smithygenerated.aws_cryptography_keystore.models.AwsKms(
+        grant_tokens=(
+            (
+                [
+                    b"".join(ord(c).to_bytes(2, "big") for c in list_element).decode(
+                        "utf-16-be"
+                    )
+                    for list_element in dafny_input.grantTokens.value
+                ]
+            )
+            if (dafny_input.grantTokens.is_Some)
+            else None
+        ),
+        kms_client=(
+            (
+                aws_cryptographic_material_providers.smithygenerated.aws_cryptography_keystore.dafny_to_smithy.aws_cryptography_keystore_KmsClientReference(
+                    dafny_input.kmsClient.UnwrapOr(None)
+                )
+            )
+            if (dafny_input.kmsClient.UnwrapOr(None) is not None)
+            else None
+        ),
+    )
 
 
 def aws_cryptography_keystore_KmsClientReference(dafny_input):
+    return dafny_input._impl
+
+
+def aws_cryptography_keystore_Storage(dafny_input):
+    # Convert Storage
+    if isinstance(dafny_input, Storage_ddb):
+        Storage_union_value = aws_cryptographic_material_providers.smithygenerated.aws_cryptography_keystore.models.StorageDdb(
+            aws_cryptographic_material_providers.smithygenerated.aws_cryptography_keystore.dafny_to_smithy.aws_cryptography_keystore_DynamoDBTable(
+                dafny_input.ddb
+            )
+        )
+    elif isinstance(dafny_input, Storage_custom):
+        Storage_union_value = aws_cryptographic_material_providers.smithygenerated.aws_cryptography_keystore.models.StorageCustom(
+            aws_cryptographic_material_providers.smithygenerated.aws_cryptography_keystore.dafny_to_smithy.aws_cryptography_keystore_KeyStorageInterfaceReference(
+                dafny_input.custom
+            )
+        )
+    else:
+        raise ValueError("No recognized union value in union type: " + str(dafny_input))
+
+    return Storage_union_value
+
+
+def aws_cryptography_keystore_DynamoDBTable(dafny_input):
+    return aws_cryptographic_material_providers.smithygenerated.aws_cryptography_keystore.models.DynamoDBTable(
+        ddb_table_name=b"".join(
+            ord(c).to_bytes(2, "big") for c in dafny_input.ddbTableName
+        ).decode("utf-16-be"),
+        ddb_client=(
+            (
+                aws_cryptographic_material_providers.smithygenerated.aws_cryptography_keystore.dafny_to_smithy.aws_cryptography_keystore_DdbClientReference(
+                    dafny_input.ddbClient.UnwrapOr(None)
+                )
+            )
+            if (dafny_input.ddbClient.UnwrapOr(None) is not None)
+            else None
+        ),
+    )
+
+
+def aws_cryptography_keystore_KeyStorageInterfaceReference(dafny_input):
+    if hasattr(dafny_input, "_native_impl"):
+        return dafny_input._native_impl
+
+    else:
+        from aws_cryptographic_material_providers.smithygenerated.aws_cryptography_keystore.references import (
+            KeyStorageInterface,
+        )
+
+        return KeyStorageInterface(_impl=dafny_input)
+
+
+def aws_cryptography_keystore_DdbClientReference(dafny_input):
     return dafny_input._impl
 
 
@@ -257,15 +528,30 @@ def aws_cryptography_keystore_KeyStoreConfig(dafny_input):
     import aws_cryptographic_material_providers.smithygenerated.aws_cryptography_keystore.config
 
     return aws_cryptographic_material_providers.smithygenerated.aws_cryptography_keystore.config.KeyStoreConfig(
-        ddb_table_name=b"".join(
-            ord(c).to_bytes(2, "big") for c in dafny_input.ddbTableName
-        ).decode("utf-16-be"),
         kms_configuration=aws_cryptographic_material_providers.smithygenerated.aws_cryptography_keystore.dafny_to_smithy.aws_cryptography_keystore_KMSConfiguration(
             dafny_input.kmsConfiguration
         ),
         logical_key_store_name=b"".join(
             ord(c).to_bytes(2, "big") for c in dafny_input.logicalKeyStoreName
         ).decode("utf-16-be"),
+        key_management=(
+            (
+                aws_cryptographic_material_providers.smithygenerated.aws_cryptography_keystore.dafny_to_smithy.aws_cryptography_keystore_KeyManagement(
+                    dafny_input.keyManagement.value
+                )
+            )
+            if (dafny_input.keyManagement.is_Some)
+            else None
+        ),
+        ddb_table_name=(
+            (
+                b"".join(
+                    ord(c).to_bytes(2, "big") for c in dafny_input.ddbTableName.value
+                ).decode("utf-16-be")
+            )
+            if (dafny_input.ddbTableName.is_Some)
+            else None
+        ),
         id=(
             (
                 b"".join(
@@ -285,6 +571,15 @@ def aws_cryptography_keystore_KeyStoreConfig(dafny_input):
                 ]
             )
             if (dafny_input.grantTokens.is_Some)
+            else None
+        ),
+        storage=(
+            (
+                aws_cryptographic_material_providers.smithygenerated.aws_cryptography_keystore.dafny_to_smithy.aws_cryptography_keystore_Storage(
+                    dafny_input.storage.value
+                )
+            )
+            if (dafny_input.storage.is_Some)
             else None
         ),
         ddb_client=(
