AwsCryptographicMaterialProviders/dafny/AwsCryptographyKeyStore/Model/AwsCryptographyKeyStoreTypes.dfy
@@ -16,6 +16,16 @@ module {:extern "software.amazon.cryptography.keystore.internaldafny.types" } Aw
 
   // Begin Generated Types
 
+  datatype ActiveHierarchicalSymmetric = | ActiveHierarchicalSymmetric (
+    nameonly Version: string
+  )
+  datatype ActiveHierarchicalSymmetricBeacon = | ActiveHierarchicalSymmetricBeacon (
+
+                                               )
+  datatype AwsKms = | AwsKms (
+    nameonly grantTokens: Option<GrantTokenList> := Option.None ,
+    nameonly kmsClient: Option<ComAmazonawsKmsTypes.IKMSClient> := Option.None
+  )
   datatype BeaconKeyMaterials = | BeaconKeyMaterials (
     nameonly beaconKeyIdentifier: string ,
     nameonly encryptionContext: EncryptionContext ,
@@ -44,7 +54,20 @@ module {:extern "software.amazon.cryptography.keystore.internaldafny.types" } Aw
   datatype Discovery = | Discovery (
 
                        )
+  datatype DynamoDBTable = | DynamoDBTable (
+    nameonly ddbTableName: ComAmazonawsDynamodbTypes.TableName ,
+    nameonly ddbClient: Option<ComAmazonawsDynamodbTypes.IDynamoDBClient> := Option.None
+  )
+  datatype EncryptedHierarchicalKey = | EncryptedHierarchicalKey (
+    nameonly Identifier: string ,
+    nameonly Type: HierarchicalKeyType ,
+    nameonly CreateTime: string ,
+    nameonly KmsArn: string ,
+    nameonly EncryptionContext: EncryptionContextString ,
+    nameonly CiphertextBlob: seq<uint8>
+  )
   type EncryptionContext = map<Utf8Bytes, Utf8Bytes>
+  type EncryptionContextString = map<string, string>
   datatype GetActiveBranchKeyInput = | GetActiveBranchKeyInput (
     nameonly branchKeyIdentifier: string
   )
@@ -64,15 +87,280 @@ module {:extern "software.amazon.cryptography.keystore.internaldafny.types" } Aw
   datatype GetBranchKeyVersionOutput = | GetBranchKeyVersionOutput (
     nameonly branchKeyMaterials: BranchKeyMaterials
   )
+  datatype GetEncryptedActiveBranchKeyInput = | GetEncryptedActiveBranchKeyInput (
+    nameonly Identifier: string
+  )
+  datatype GetEncryptedActiveBranchKeyOutput = | GetEncryptedActiveBranchKeyOutput (
+    nameonly Item: EncryptedHierarchicalKey
+  )
+  datatype GetEncryptedBeaconKeyInput = | GetEncryptedBeaconKeyInput (
+    nameonly Identifier: string
+  )
+  datatype GetEncryptedBeaconKeyOutput = | GetEncryptedBeaconKeyOutput (
+    nameonly Item: EncryptedHierarchicalKey
+  )
+  datatype GetEncryptedBranchKeyVersionInput = | GetEncryptedBranchKeyVersionInput (
+    nameonly Identifier: string ,
+    nameonly Version: string
+  )
+  datatype GetEncryptedBranchKeyVersionOutput = | GetEncryptedBranchKeyVersionOutput (
+    nameonly Item: EncryptedHierarchicalKey
+  )
+  datatype GetKeyStorageInfoInput = | GetKeyStorageInfoInput (
+
+                                    )
+  datatype GetKeyStorageInfoOutput = | GetKeyStorageInfoOutput (
+    nameonly Name: Utf8Bytes ,
+    nameonly LogicalName: Utf8Bytes
+  )
   datatype GetKeyStoreInfoOutput = | GetKeyStoreInfoOutput (
     nameonly keyStoreId: string ,
-    nameonly keyStoreName: ComAmazonawsDynamodbTypes.TableName ,
+    nameonly keyStoreName: string ,
     nameonly logicalKeyStoreName: string ,
     nameonly grantTokens: GrantTokenList ,
     nameonly kmsConfiguration: KMSConfiguration
   )
   type GrantTokenList = seq<string>
+  datatype HierarchicalKeyType =
+    | ActiveHierarchicalSymmetricVersion(ActiveHierarchicalSymmetricVersion: ActiveHierarchicalSymmetric)
+    | HierarchicalSymmetricVersion(HierarchicalSymmetricVersion: HierarchicalSymmetric)
+    | ActiveHierarchicalSymmetricBeacon(ActiveHierarchicalSymmetricBeacon: ActiveHierarchicalSymmetricBeacon)
+  datatype HierarchicalSymmetric = | HierarchicalSymmetric (
+    nameonly Version: string
+  )
   type HmacKeyMap = map<string, Secret>
+  datatype KeyManagement =
+    | kms(kms: AwsKms)
+  class IKeyStorageInterfaceCallHistory {
+    ghost constructor() {
+      GetEncryptedActiveBranchKey := [];
+      WriteNewEncryptedBranchKey := [];
+      WriteNewEncryptedBranchKeyVersion := [];
+      GetKeyStorageInfo := [];
+      GetEncryptedBranchKeyVersion := [];
+      GetEncryptedBeaconKey := [];
+    }
+    ghost var GetEncryptedActiveBranchKey: seq<DafnyCallEvent<GetEncryptedActiveBranchKeyInput, Result<GetEncryptedActiveBranchKeyOutput, Error>>>
+    ghost var WriteNewEncryptedBranchKey: seq<DafnyCallEvent<WriteNewEncryptedBranchKeyInput, Result<WriteNewEncryptedBranchKeyOutput, Error>>>
+    ghost var WriteNewEncryptedBranchKeyVersion: seq<DafnyCallEvent<WriteNewEncryptedBranchKeyVersionInput, Result<WriteNewEncryptedBranchKeyVersionOutput, Error>>>
+    ghost var GetKeyStorageInfo: seq<DafnyCallEvent<GetKeyStorageInfoInput, Result<GetKeyStorageInfoOutput, Error>>>
+    ghost var GetEncryptedBranchKeyVersion: seq<DafnyCallEvent<GetEncryptedBranchKeyVersionInput, Result<GetEncryptedBranchKeyVersionOutput, Error>>>
+    ghost var GetEncryptedBeaconKey: seq<DafnyCallEvent<GetEncryptedBeaconKeyInput, Result<GetEncryptedBeaconKeyOutput, Error>>>
+  }
+  trait {:termination false} IKeyStorageInterface
+  {
+    // Helper to define any additional modifies/reads clauses.
+    // If your operations need to mutate state,
+    // add it in your constructor function:
+    // Modifies := {your, fields, here, History};
+    // If you do not need to mutate anything:
+    // Modifies := {History};
+
+    ghost const Modifies: set<object>
+    // For an unassigned field defined in a trait,
+    // Dafny can only assign a value in the constructor.
+    // This means that for Dafny to reason about this value,
+    // it needs some way to know (an invariant),
+    // about the state of the object.
+    // This builds on the Valid/Repr paradigm
+    // To make this kind requires safe to add
+    // to methods called from unverified code,
+    // the predicate MUST NOT take any arguments.
+    // This means that the correctness of this requires
+    // MUST only be evaluated by the class itself.
+    // If you require any additional mutation,
+    // then you MUST ensure everything you need in ValidState.
+    // You MUST also ensure ValidState in your constructor.
+    predicate ValidState()
+      ensures ValidState() ==> History in Modifies
+    ghost const History: IKeyStorageInterfaceCallHistory
+    predicate GetEncryptedActiveBranchKeyEnsuresPublicly(input: GetEncryptedActiveBranchKeyInput , output: Result<GetEncryptedActiveBranchKeyOutput, Error>)
+    // The public method to be called by library consumers
+    method GetEncryptedActiveBranchKey ( input: GetEncryptedActiveBranchKeyInput )
+      returns (output: Result<GetEncryptedActiveBranchKeyOutput, Error>)
+      requires
+        && ValidState()
+      modifies Modifies - {History} ,
+               History`GetEncryptedActiveBranchKey
+      // Dafny will skip type parameters when generating a default decreases clause.
+      decreases Modifies - {History}
+      ensures
+        && ValidState()
+      ensures GetEncryptedActiveBranchKeyEnsuresPublicly(input, output)
+      ensures History.GetEncryptedActiveBranchKey == old(History.GetEncryptedActiveBranchKey) + [DafnyCallEvent(input, output)]
+    {
+      output := GetEncryptedActiveBranchKey' (input);
+      History.GetEncryptedActiveBranchKey := History.GetEncryptedActiveBranchKey + [DafnyCallEvent(input, output)];
+    }
+    // The method to implement in the concrete class.
+    method GetEncryptedActiveBranchKey' ( input: GetEncryptedActiveBranchKeyInput )
+      returns (output: Result<GetEncryptedActiveBranchKeyOutput, Error>)
+      requires
+        && ValidState()
+      modifies Modifies - {History}
+      // Dafny will skip type parameters when generating a default decreases clause.
+      decreases Modifies - {History}
+      ensures
+        && ValidState()
+      ensures GetEncryptedActiveBranchKeyEnsuresPublicly(input, output)
+      ensures unchanged(History)
+
+    predicate WriteNewEncryptedBranchKeyEnsuresPublicly(input: WriteNewEncryptedBranchKeyInput , output: Result<WriteNewEncryptedBranchKeyOutput, Error>)
+    // The public method to be called by library consumers
+    method WriteNewEncryptedBranchKey ( input: WriteNewEncryptedBranchKeyInput )
+      returns (output: Result<WriteNewEncryptedBranchKeyOutput, Error>)
+      requires
+        && ValidState()
+      modifies Modifies - {History} ,
+               History`WriteNewEncryptedBranchKey
+      // Dafny will skip type parameters when generating a default decreases clause.
+      decreases Modifies - {History}
+      ensures
+        && ValidState()
+      ensures WriteNewEncryptedBranchKeyEnsuresPublicly(input, output)
+      ensures History.WriteNewEncryptedBranchKey == old(History.WriteNewEncryptedBranchKey) + [DafnyCallEvent(input, output)]
+    {
+      output := WriteNewEncryptedBranchKey' (input);
+      History.WriteNewEncryptedBranchKey := History.WriteNewEncryptedBranchKey + [DafnyCallEvent(input, output)];
+    }
+    // The method to implement in the concrete class.
+    method WriteNewEncryptedBranchKey' ( input: WriteNewEncryptedBranchKeyInput )
+      returns (output: Result<WriteNewEncryptedBranchKeyOutput, Error>)
+      requires
+        && ValidState()
+      modifies Modifies - {History}
+      // Dafny will skip type parameters when generating a default decreases clause.
+      decreases Modifies - {History}
+      ensures
+        && ValidState()
+      ensures WriteNewEncryptedBranchKeyEnsuresPublicly(input, output)
+      ensures unchanged(History)
+
+    predicate WriteNewEncryptedBranchKeyVersionEnsuresPublicly(input: WriteNewEncryptedBranchKeyVersionInput , output: Result<WriteNewEncryptedBranchKeyVersionOutput, Error>)
+    // The public method to be called by library consumers
+    method WriteNewEncryptedBranchKeyVersion ( input: WriteNewEncryptedBranchKeyVersionInput )
+      returns (output: Result<WriteNewEncryptedBranchKeyVersionOutput, Error>)
+      requires
+        && ValidState()
+      modifies Modifies - {History} ,
+               History`WriteNewEncryptedBranchKeyVersion
+      // Dafny will skip type parameters when generating a default decreases clause.
+      decreases Modifies - {History}
+      ensures
+        && ValidState()
+      ensures WriteNewEncryptedBranchKeyVersionEnsuresPublicly(input, output)
+      ensures History.WriteNewEncryptedBranchKeyVersion == old(History.WriteNewEncryptedBranchKeyVersion) + [DafnyCallEvent(input, output)]
+    {
+      output := WriteNewEncryptedBranchKeyVersion' (input);
+      History.WriteNewEncryptedBranchKeyVersion := History.WriteNewEncryptedBranchKeyVersion + [DafnyCallEvent(input, output)];
+    }
+    // The method to implement in the concrete class.
+    method WriteNewEncryptedBranchKeyVersion' ( input: WriteNewEncryptedBranchKeyVersionInput )
+      returns (output: Result<WriteNewEncryptedBranchKeyVersionOutput, Error>)
+      requires
+        && ValidState()
+      modifies Modifies - {History}
+      // Dafny will skip type parameters when generating a default decreases clause.
+      decreases Modifies - {History}
+      ensures
+        && ValidState()
+      ensures WriteNewEncryptedBranchKeyVersionEnsuresPublicly(input, output)
+      ensures unchanged(History)
+
+    predicate GetKeyStorageInfoEnsuresPublicly(input: GetKeyStorageInfoInput , output: Result<GetKeyStorageInfoOutput, Error>)
+    // The public method to be called by library consumers
+    method GetKeyStorageInfo ( input: GetKeyStorageInfoInput )
+      returns (output: Result<GetKeyStorageInfoOutput, Error>)
+      requires
+        && ValidState()
+      modifies Modifies - {History} ,
+               History`GetKeyStorageInfo
+      // Dafny will skip type parameters when generating a default decreases clause.
+      decreases Modifies - {History}
+      ensures
+        && ValidState()
+      ensures GetKeyStorageInfoEnsuresPublicly(input, output)
+      ensures History.GetKeyStorageInfo == old(History.GetKeyStorageInfo) + [DafnyCallEvent(input, output)]
+    {
+      output := GetKeyStorageInfo' (input);
+      History.GetKeyStorageInfo := History.GetKeyStorageInfo + [DafnyCallEvent(input, output)];
+    }
+    // The method to implement in the concrete class.
+    method GetKeyStorageInfo' ( input: GetKeyStorageInfoInput )
+      returns (output: Result<GetKeyStorageInfoOutput, Error>)
+      requires
+        && ValidState()
+      modifies Modifies - {History}
+      // Dafny will skip type parameters when generating a default decreases clause.
+      decreases Modifies - {History}
+      ensures
+        && ValidState()
+      ensures GetKeyStorageInfoEnsuresPublicly(input, output)
+      ensures unchanged(History)
+
+    predicate GetEncryptedBranchKeyVersionEnsuresPublicly(input: GetEncryptedBranchKeyVersionInput , output: Result<GetEncryptedBranchKeyVersionOutput, Error>)
+    // The public method to be called by library consumers
+    method GetEncryptedBranchKeyVersion ( input: GetEncryptedBranchKeyVersionInput )
+      returns (output: Result<GetEncryptedBranchKeyVersionOutput, Error>)
+      requires
+        && ValidState()
+      modifies Modifies - {History} ,
+               History`GetEncryptedBranchKeyVersion
+      // Dafny will skip type parameters when generating a default decreases clause.
+      decreases Modifies - {History}
+      ensures
+        && ValidState()
+      ensures GetEncryptedBranchKeyVersionEnsuresPublicly(input, output)
+      ensures History.GetEncryptedBranchKeyVersion == old(History.GetEncryptedBranchKeyVersion) + [DafnyCallEvent(input, output)]
+    {
+      output := GetEncryptedBranchKeyVersion' (input);
+      History.GetEncryptedBranchKeyVersion := History.GetEncryptedBranchKeyVersion + [DafnyCallEvent(input, output)];
+    }
+    // The method to implement in the concrete class.
+    method GetEncryptedBranchKeyVersion' ( input: GetEncryptedBranchKeyVersionInput )
+      returns (output: Result<GetEncryptedBranchKeyVersionOutput, Error>)
+      requires
+        && ValidState()
+      modifies Modifies - {History}
+      // Dafny will skip type parameters when generating a default decreases clause.
+      decreases Modifies - {History}
+      ensures
+        && ValidState()
+      ensures GetEncryptedBranchKeyVersionEnsuresPublicly(input, output)
+      ensures unchanged(History)
+
+    predicate GetEncryptedBeaconKeyEnsuresPublicly(input: GetEncryptedBeaconKeyInput , output: Result<GetEncryptedBeaconKeyOutput, Error>)
+    // The public method to be called by library consumers
+    method GetEncryptedBeaconKey ( input: GetEncryptedBeaconKeyInput )
+      returns (output: Result<GetEncryptedBeaconKeyOutput, Error>)
+      requires
+        && ValidState()
+      modifies Modifies - {History} ,
+               History`GetEncryptedBeaconKey
+      // Dafny will skip type parameters when generating a default decreases clause.
+      decreases Modifies - {History}
+      ensures
+        && ValidState()
+      ensures GetEncryptedBeaconKeyEnsuresPublicly(input, output)
+      ensures History.GetEncryptedBeaconKey == old(History.GetEncryptedBeaconKey) + [DafnyCallEvent(input, output)]
+    {
+      output := GetEncryptedBeaconKey' (input);
+      History.GetEncryptedBeaconKey := History.GetEncryptedBeaconKey + [DafnyCallEvent(input, output)];
+    }
+    // The method to implement in the concrete class.
+    method GetEncryptedBeaconKey' ( input: GetEncryptedBeaconKeyInput )
+      returns (output: Result<GetEncryptedBeaconKeyOutput, Error>)
+      requires
+        && ValidState()
+      modifies Modifies - {History}
+      // Dafny will skip type parameters when generating a default decreases clause.
+      decreases Modifies - {History}
+      ensures
+        && ValidState()
+      ensures GetEncryptedBeaconKeyEnsuresPublicly(input, output)
+      ensures unchanged(History)
+
+  }
   class IKeyStoreClientCallHistory {
     ghost constructor() {
       GetKeyStoreInfo := [];
@@ -225,11 +513,13 @@ module {:extern "software.amazon.cryptography.keystore.internaldafny.types" } Aw
 
   }
   datatype KeyStoreConfig = | KeyStoreConfig (
-    nameonly ddbTableName: ComAmazonawsDynamodbTypes.TableName ,
     nameonly kmsConfiguration: KMSConfiguration ,
     nameonly logicalKeyStoreName: string ,
+    nameonly keyManagement: Option<KeyManagement> := Option.None ,
+    nameonly ddbTableName: Option<ComAmazonawsDynamodbTypes.TableName> := Option.None ,
     nameonly id: Option<string> := Option.None ,
     nameonly grantTokens: Option<GrantTokenList> := Option.None ,
+    nameonly storage: Option<Storage> := Option.None ,
     nameonly ddbClient: Option<ComAmazonawsDynamodbTypes.IDynamoDBClient> := Option.None ,
     nameonly kmsClient: Option<ComAmazonawsKmsTypes.IKMSClient> := Option.None
   )
@@ -242,6 +532,9 @@ module {:extern "software.amazon.cryptography.keystore.internaldafny.types" } Aw
     nameonly region: ComAmazonawsKmsTypes.RegionType
   )
   type Secret = seq<uint8>
+  datatype Storage =
+    | ddb(ddb: DynamoDBTable)
+    | custom(custom: IKeyStorageInterface)
   type Utf8Bytes = ValidUTF8Bytes
   datatype VersionKeyInput = | VersionKeyInput (
     nameonly branchKeyIdentifier: string
@@ -249,6 +542,22 @@ module {:extern "software.amazon.cryptography.keystore.internaldafny.types" } Aw
   datatype VersionKeyOutput = | VersionKeyOutput (
 
                               )
+  datatype WriteNewEncryptedBranchKeyInput = | WriteNewEncryptedBranchKeyInput (
+    nameonly Active: EncryptedHierarchicalKey ,
+    nameonly Version: EncryptedHierarchicalKey ,
+    nameonly Beacon: EncryptedHierarchicalKey
+  )
+  datatype WriteNewEncryptedBranchKeyOutput = | WriteNewEncryptedBranchKeyOutput (
+
+                                              )
+  datatype WriteNewEncryptedBranchKeyVersionInput = | WriteNewEncryptedBranchKeyVersionInput (
+    nameonly Active: EncryptedHierarchicalKey ,
+    nameonly Version: EncryptedHierarchicalKey ,
+    nameonly oldActive: EncryptedHierarchicalKey
+  )
+  datatype WriteNewEncryptedBranchKeyVersionOutput = | WriteNewEncryptedBranchKeyVersionOutput (
+
+                                                     )
   datatype Error =
       // Local Error structures are listed here
     | KeyStoreException (
@@ -302,17 +611,47 @@ abstract module AbstractAwsCryptographyKeyStoreService
   import opened Types = AwsCryptographyKeyStoreTypes
   import Operations : AbstractAwsCryptographyKeyStoreOperations
   function method DefaultKeyStoreConfig(): KeyStoreConfig
-  method KeyStore(config: KeyStoreConfig := DefaultKeyStoreConfig())
+  method {:isoluate_asserations} {:resource_limit 94000000 } KeyStore(config: KeyStoreConfig := DefaultKeyStoreConfig())
     returns (res: Result<KeyStoreClient, Error>)
     requires config.ddbClient.Some? ==>
                config.ddbClient.value.ValidState()
     requires config.kmsClient.Some? ==>
                config.kmsClient.value.ValidState()
+    requires config.storage.Some? ==>
+               config.storage.value.custom? ==>
+                 config.storage.value.custom.ValidState()
+    requires config.keyManagement.Some? ==>
+               config.keyManagement.value.kms? ==>
+                 config.keyManagement.value.kms.kmsClient.Some? ==>
+                   config.keyManagement.value.kms.kmsClient.value.ValidState()
+    requires config.storage.Some? ==>
+               config.storage.value.ddb? ==>
+                 config.storage.value.ddb.ddbClient.Some? ==>
+                   config.storage.value.ddb.ddbClient.value.ValidState()
     modifies if config.ddbClient.Some? then
                config.ddbClient.value.Modifies
              else {}
     modifies if config.kmsClient.Some? then
                config.kmsClient.value.Modifies
+             else {}
+    modifies if config.storage.Some? then
+               if config.storage.value.custom? then
+                 config.storage.value.custom.Modifies
+               else {}
+             else {}
+    modifies if config.keyManagement.Some? then
+               if config.keyManagement.value.kms? then
+                 if config.keyManagement.value.kms.kmsClient.Some? then
+                   config.keyManagement.value.kms.kmsClient.value.Modifies
+                 else {}
+               else {}
+             else {}
+    modifies if config.storage.Some? then
+               if config.storage.value.ddb? then
+                 if config.storage.value.ddb.ddbClient.Some? then
+                   config.storage.value.ddb.ddbClient.value.Modifies
+                 else {}
+               else {}
              else {}
     ensures res.Success? ==>
               && fresh(res.value)
@@ -323,6 +662,25 @@ abstract module AbstractAwsCryptographyKeyStoreService
                        ) - ( if config.kmsClient.Some? then
                                config.kmsClient.value.Modifies
                              else {}
+                       ) - ( if config.storage.Some? then
+                               if config.storage.value.custom? then
+                                 config.storage.value.custom.Modifies
+                               else {}
+                             else {}
+                       ) - ( if config.keyManagement.Some? then
+                               if config.keyManagement.value.kms? then
+                                 if config.keyManagement.value.kms.kmsClient.Some? then
+                                   config.keyManagement.value.kms.kmsClient.value.Modifies
+                                 else {}
+                               else {}
+                             else {}
+                       ) - ( if config.storage.Some? then
+                               if config.storage.value.ddb? then
+                                 if config.storage.value.ddb.ddbClient.Some? then
+                                   config.storage.value.ddb.ddbClient.value.Modifies
+                                 else {}
+                               else {}
+                             else {}
                        ) )
               && fresh(res.value.History)
               && res.value.ValidState()
@@ -330,6 +688,17 @@ abstract module AbstractAwsCryptographyKeyStoreService
               config.ddbClient.value.ValidState()
     ensures config.kmsClient.Some? ==>
               config.kmsClient.value.ValidState()
+    ensures config.storage.Some? ==>
+              config.storage.value.custom? ==>
+                config.storage.value.custom.ValidState()
+    ensures config.keyManagement.Some? ==>
+              config.keyManagement.value.kms? ==>
+                config.keyManagement.value.kms.kmsClient.Some? ==>
+                  config.keyManagement.value.kms.kmsClient.value.ValidState()
+    ensures config.storage.Some? ==>
+              config.storage.value.ddb? ==>
+                config.storage.value.ddb.ddbClient.Some? ==>
+                  config.storage.value.ddb.ddbClient.value.ValidState()
 
   // Helper functions for the benefit of native code to create a Success(client) without referring to Dafny internals
   function method CreateSuccessOfClient(client: IKeyStoreClient): Result<IKeyStoreClient, Error> {
