AwsCryptographicMaterialProviders/dafny/AwsCryptographyKeyStore/src/CreateKeys.dfy
@@ -3,7 +3,7 @@
 
 include "../Model/AwsCryptographyKeyStoreTypes.dfy"
 include "Structure.dfy"
-include "DDBKeystoreOperations.dfy"
+include "DefaultKeyStorageInterface.dfy"
 include "KMSKeystoreOperations.dfy"
 include "ErrorMessages.dfy"
 include "../../AwsCryptographicMaterialProviders/src/AwsArnParsing.dfy"
@@ -12,10 +12,9 @@ include "KmsArn.dfy"
 module {:options "/functionSyntax:4" } CreateKeys {
   import opened StandardLibrary
   import opened Wrappers
-
   import Structure
+  import DefaultKeyStorageInterface
   import KMSKeystoreOperations
-  import DDBKeystoreOperations
   import ErrorMessages = KeyStoreErrorMessages
 
   import opened Seq
@@ -32,30 +31,27 @@ module {:options "/functionSyntax:4" } CreateKeys {
   //#
   //# - `branchKeyId`: The identifier
   //# - `encryptionContext`: Additional encryption context to bind to the created keys
-
-  //  - `kmsKeyArn`: KMS key ARN used to create keys
-  method {:vcs_split_on_every_assert} CreateBranchAndBeaconKeys(
+  method CreateBranchAndBeaconKeys(
     branchKeyIdentifier: string,
     customEncryptionContext: map<string, string>,
     timestamp: string,
     branchKeyVersion: string,
-    ddbTableName: DDB.TableName,
     logicalKeyStoreName: string,
     kmsConfiguration: Types.KMSConfiguration,
     grantTokens: KMS.GrantTokenList,
     kmsClient: KMS.IKMSClient,
-    ddbClient: DDB.IDynamoDBClient
+    storage: Types.IKeyStorageInterface
   )
     returns (output: Result<Types.CreateKeyOutput, Types.Error>)
     requires 0 < |branchKeyIdentifier|
     requires 0 < |branchKeyVersion|
     requires forall k <- customEncryptionContext :: DDB.IsValid_AttributeName(Structure.ENCRYPTION_CONTEXT_PREFIX + k)
-    requires ddbClient.Modifies !! kmsClient.Modifies
+    requires storage.Modifies !! kmsClient.Modifies
     requires KMSKeystoreOperations.HasKeyId(kmsConfiguration) && KmsArn.ValidKmsArn?(KMSKeystoreOperations.GetKeyId(kmsConfiguration))
 
-    requires kmsClient.ValidState() && ddbClient.ValidState()
-    modifies ddbClient.Modifies, kmsClient.Modifies
-    ensures ddbClient.ValidState() && kmsClient.ValidState()
+    requires kmsClient.ValidState() && storage.ValidState()
+    modifies storage.Modifies, kmsClient.Modifies
+    ensures storage.ValidState() && kmsClient.ValidState()
 
     //= aws-encryption-sdk-specification/framework/branch-key-store.md#createkey
     //= type=implication
@@ -66,14 +62,12 @@ module {:options "/functionSyntax:4" } CreateKeys {
 
               //= aws-encryption-sdk-specification/framework/branch-key-store.md#branch-key-and-beacon-key-creation
               //= type=implication
-              //# The operation MUST call [AWS KMS API GenerateDataKeyWithoutPlaintext](https://docs.aws.amazon.com/kms/latest/APIReference/API_GenerateDataKeyWithoutPlaintext.html).
-
-              //= aws-encryption-sdk-specification/framework/branch-key-store.md#branch-key-and-beacon-key-creation
-              //= type=implication
               //# The call to AWS KMS GenerateDataKeyWithoutPlaintext MUST use the configured AWS KMS client to make the call.
+              // The second call is for the beacon key, the first call is the decrypt only. See Seq.Last(Seq.DropLast(
               && |kmsClient.History.GenerateDataKeyWithoutPlaintext| == |old(kmsClient.History.GenerateDataKeyWithoutPlaintext)| + 2
-
               && |kmsClient.History.ReEncrypt| == |old(kmsClient.History.ReEncrypt)| + 1
+              && old(kmsClient.History.GenerateDataKeyWithoutPlaintext) < kmsClient.History.GenerateDataKeyWithoutPlaintext
+              && old(kmsClient.History.ReEncrypt) < kmsClient.History.ReEncrypt
 
               && var decryptOnlyEncryptionContext := Structure.DecryptOnlyBranchKeyEncryptionContext(
                                                        branchKeyIdentifier,
@@ -89,6 +83,16 @@ module {:options "/functionSyntax:4" } CreateKeys {
               //# The logical keystore name MUST be bound to every created key.
               && decryptOnlyEncryptionContext[Structure.TABLE_FIELD] == logicalKeyStoreName
 
+              //= aws-encryption-sdk-specification/framework/branch-key-store.md#encryption-context
+              //= type=implication
+              //# Any additionally attributes in the EncryptionContext
+              //# of the [encrypted hierarchical key](./key-store/key-storage.md#encryptedhierarchicalkey)
+              //# MUST be added to the encryption context.
+              && (forall k <- customEncryptionContext
+                    ::
+                      && Structure.ENCRYPTION_CONTEXT_PREFIX + k in decryptOnlyEncryptionContext
+                      && decryptOnlyEncryptionContext[Structure.ENCRYPTION_CONTEXT_PREFIX + k] == customEncryptionContext[k])
+
               //= aws-encryption-sdk-specification/framework/branch-key-store.md#branch-key-and-beacon-key-creation
               //= type=implication
               //# The wrapped Branch Keys, DECRYPT_ONLY and ACTIVE, MUST be created according to [Wrapped Branch Key Creation](#wrapped-branch-key-creation).
@@ -101,10 +105,16 @@ module {:options "/functionSyntax:4" } CreateKeys {
                    decryptOnlyEncryptionContext
                  )
 
+
+              //= aws-encryption-sdk-specification/framework/branch-key-store.md#branch-key-and-beacon-key-creation
+              //= type=implication
+              //# The operation MUST call [AWS KMS API GenerateDataKeyWithoutPlaintext](https://docs.aws.amazon.com/kms/latest/APIReference/API_GenerateDataKeyWithoutPlaintext.html).
+              && var beaconKmsRequest := Seq.Last(kmsClient.History.GenerateDataKeyWithoutPlaintext);
+
               //= aws-encryption-sdk-specification/framework/branch-key-store.md#branch-key-and-beacon-key-creation
               //= type=implication
               //# The operation MUST call AWS KMS GenerateDataKeyWithoutPlaintext with a request constructed as follows:
-              && var beaconKmsInput := Seq.Last(kmsClient.History.GenerateDataKeyWithoutPlaintext).input;
+              && var beaconKmsInput := beaconKmsRequest.input;
 
               //= aws-encryption-sdk-specification/framework/branch-key-store.md#branch-key-and-beacon-key-creation
               //= type=implication
@@ -126,81 +136,71 @@ module {:options "/functionSyntax:4" } CreateKeys {
               //# - `GrantTokens` MUST be this keystore's [grant tokens](https://docs.aws.amazon.com/kms/latest/developerguide/concepts.html#grant_token).
               && beaconKmsInput.GrantTokens == Some(grantTokens)
 
-              //= aws-encryption-sdk-specification/framework/branch-key-store.md#createkey
-              //= type=implication
-              //# If creation of the keys are successful,
-              //# the operation MUST call Amazon DynamoDB TransactWriteItems according to the [write key material](#writing-branch-key-and-beacon-key-to-key-store) section.
+              && beaconKmsRequest.output.Success?
+              && beaconKmsRequest.output.value.CiphertextBlob.Some?
 
-              && Seq.Last(kmsClient.History.GenerateDataKeyWithoutPlaintext).output.Success?
-              && var beaconKmsOutput := Seq.Last(kmsClient.History.GenerateDataKeyWithoutPlaintext).output.value;
-              && beaconKmsOutput.CiphertextBlob.Some?
+              && |storage.History.WriteNewEncryptedBranchKey| == |old(storage.History.WriteNewEncryptedBranchKey)| + 1
 
-              //= aws-encryption-sdk-specification/framework/branch-key-store.md#writing-branch-key-and-beacon-key-to-keystore
-              //= type=implication
-              //# To add the branch keys and a beacon key to the keystore the
-              //# operation MUST call [Amazon DynamoDB API TransactWriteItems](https://docs.aws.amazon.com/amazondynamodb/latest/APIReference/API_TransactWriteItems.html).
-
-              //= aws-encryption-sdk-specification/framework/branch-key-store.md#writing-branch-key-and-beacon-key-to-keystore
-              //= type=implication
-              //# The call to Amazon DynamoDB TransactWriteItems MUST use the configured Amazon DynamoDB Client to make the call.
-
-              && |ddbClient.History.TransactWriteItems| == |old(ddbClient.History.TransactWriteItems)| + 1
-
-              //= aws-encryption-sdk-specification/framework/branch-key-store.md#writing-branch-key-and-beacon-key-to-keystore
-              //= type=implication
-              //# The operation MUST call Amazon DynamoDB TransactWriteItems with a request constructed as follows:
-              && var writeNewKey := Seq.Last(ddbClient.History.TransactWriteItems).input;
-
-              && 3 == |writeNewKey.TransactItems|
-
-              //= aws-encryption-sdk-specification/framework/branch-key-store.md#writing-branch-key-and-beacon-key-to-keystore
-              //= type=implication
-              //# - Every key-value pair of the custom [encryption context](./structures.md#encryption-context-3) that is associated with the branch key
-              //# MUST be added with an Attribute Name of `aws-crypto-ec:` + the Key and Attribute Value (S) of the value.
-              && (forall k <- customEncryptionContext ::
-                    && Structure.ENCRYPTION_CONTEXT_PREFIX + k in decryptOnlyEncryptionContext
-                    && decryptOnlyEncryptionContext[Structure.ENCRYPTION_CONTEXT_PREFIX + k] == customEncryptionContext[k])
-
-              && writeNewKey.TransactItems[0].Put.Some?
-              && writeNewKey.TransactItems[0].Put.value.Item
-                 == Structure.ToAttributeMap(
-                      decryptOnlyEncryptionContext,
-                      //= aws-encryption-sdk-specification/framework/branch-key-store.md#wrapped-branch-key-creation
-                      //= type=implication
-                      //# If the call to AWS KMS GenerateDataKeyWithoutPlaintext succeeds,
-                      //# the operation MUST use the GenerateDataKeyWithoutPlaintext result `CiphertextBlob`
-                      //# as the wrapped DECRYPT_ONLY Branch Key.
-                      Seq.Last(Seq.DropLast(kmsClient.History.GenerateDataKeyWithoutPlaintext)).output.value.CiphertextBlob.value)
-
-              && writeNewKey.TransactItems[1].Put.Some?
-              && writeNewKey.TransactItems[1].Put.value.Item
-                 == Structure.ToAttributeMap(
-                      Structure.ActiveBranchKeyEncryptionContext(decryptOnlyEncryptionContext),
+              && Seq.Last(storage.History.WriteNewEncryptedBranchKey).input.Active
+                 == Structure.ConstructEncryptedHierarchicalKey(
+                      Seq.Last(kmsClient.History.ReEncrypt).input.DestinationEncryptionContext.value,
                       //= aws-encryption-sdk-specification/framework/branch-key-store.md#wrapped-branch-key-creation
                       //= type=implication
                       //# If the call to AWS KMS ReEncrypt succeeds,
                       //# the operation MUST use the ReEncrypt result `CiphertextBlob`
                       //# as the wrapped ACTIVE Branch Key.
-                      Seq.Last(kmsClient.History.ReEncrypt).output.value.CiphertextBlob.value)
+                      Seq.Last(kmsClient.History.ReEncrypt).output.value.CiphertextBlob.value
+                    )
 
-              && writeNewKey.TransactItems[2].Put.Some?
-              && writeNewKey.TransactItems[2].Put.value.Item
-                 == Structure.ToAttributeMap(
-                      Structure.BeaconKeyEncryptionContext(decryptOnlyEncryptionContext),
+              && Seq.Last(storage.History.WriteNewEncryptedBranchKey).input.Version
+                 == Structure.ConstructEncryptedHierarchicalKey(
+                      Seq.Last(Seq.DropLast(kmsClient.History.GenerateDataKeyWithoutPlaintext)).input.EncryptionContext.value,
+                      //= aws-encryption-sdk-specification/framework/branch-key-store.md#wrapped-branch-key-creation
+                      //= type=implication
+                      //# If the call to AWS KMS GenerateDataKeyWithoutPlaintext succeeds,
+                      //# the operation MUST use the GenerateDataKeyWithoutPlaintext result `CiphertextBlob`
+                      //# as the wrapped DECRYPT_ONLY Branch Key.
+                      Seq.Last(Seq.DropLast(kmsClient.History.GenerateDataKeyWithoutPlaintext)).output.value.CiphertextBlob.value
+                    )
+
+              && Seq.Last(storage.History.WriteNewEncryptedBranchKey).input.Beacon
+                 == Structure.ConstructEncryptedHierarchicalKey(
+                      Seq.Last(kmsClient.History.GenerateDataKeyWithoutPlaintext).input.EncryptionContext.value,
                       //= aws-encryption-sdk-specification/framework/branch-key-store.md#branch-key-and-beacon-key-creation
                       //= type=implication
                       //# If the call to AWS KMS GenerateDataKeyWithoutPlaintext succeeds,
                       //# the operation MUST use the `CiphertextBlob` as the wrapped Beacon Key.
-                      beaconKmsOutput.CiphertextBlob.value)
+                      Seq.Last(kmsClient.History.GenerateDataKeyWithoutPlaintext).output.value.CiphertextBlob.value
+                    )
 
-              && Seq.Last(ddbClient.History.TransactWriteItems).output.Success?
+              && Seq.Last(storage.History.WriteNewEncryptedBranchKey).output.Success?
 
-              //= aws-encryption-sdk-specification/framework/branch-key-store.md#createkey
-              //= type=implication
-              //# If writing to the keystore succeeds,
-              //# the operation MUST return the branch-key-id that maps to both
-              //# the branch key and the beacon key.
-              && output.value.branchKeyIdentifier == branchKeyIdentifier
+    //= aws-encryption-sdk-specification/framework/branch-key-store.md#createkey
+    //= type=implication
+    //# If creation of the keys are successful,
+    //# then the key store MUST call the configured [KeyStorage interface's](./key-store/key-storage.md#interface)
+    //# [WriteNewEncryptedBranchKey](./key-store/key-storage.md#writenewencryptedbranchkey) with these 3 [EncryptedHierarchicalKeys](./key-store/key-storage.md#encryptedhierarchicalkey).
+    ensures
+      && output.Success?
+      && |kmsClient.History.GenerateDataKeyWithoutPlaintext| == |old(kmsClient.History.GenerateDataKeyWithoutPlaintext)| + 2
+      && |kmsClient.History.ReEncrypt| == |old(kmsClient.History.ReEncrypt)| + 1
+      && Seq.Last(Seq.DropLast(kmsClient.History.GenerateDataKeyWithoutPlaintext)).output.Success?
+      && Seq.Last(kmsClient.History.GenerateDataKeyWithoutPlaintext).output.Success?
+      && Seq.Last(kmsClient.History.ReEncrypt).output.Success?
+      ==>
+        && |storage.History.WriteNewEncryptedBranchKey| == |old(storage.History.WriteNewEncryptedBranchKey)| + 1
+
+    //= aws-encryption-sdk-specification/framework/branch-key-store.md#createkey
+    //= type=implication
+    //# If writing to the keystore succeeds,
+    //# the operation MUST return the branch-key-id that maps to both
+    //# the branch key and the beacon key.
+    ensures
+      && |storage.History.WriteNewEncryptedBranchKey| == |old(storage.History.WriteNewEncryptedBranchKey)| + 1
+      && Seq.Last(storage.History.WriteNewEncryptedBranchKey).output.Success?
+      ==>
+        && output.Success?
+        && output.value.branchKeyIdentifier == branchKeyIdentifier
 
 
     //= aws-encryption-sdk-specification/framework/branch-key-store.md#createkey
@@ -220,8 +220,8 @@ module {:options "/functionSyntax:4" } CreateKeys {
           && Seq.Last(kmsClient.History.GenerateDataKeyWithoutPlaintext).output.Failure?
           ==> output.Failure?)
 
-      || (&& |ddbClient.History.TransactWriteItems| == |old(ddbClient.History.TransactWriteItems)| + 1
-          && Seq.Last(ddbClient.History.TransactWriteItems).output.Failure?
+      || (&& |storage.History.WriteNewEncryptedBranchKey| == |old(storage.History.WriteNewEncryptedBranchKey)| + 1
+          && Seq.Last(storage.History.WriteNewEncryptedBranchKey).output.Failure?
           ==> output.Failure?)
 
   {
@@ -237,16 +237,14 @@ module {:options "/functionSyntax:4" } CreateKeys {
     var activeEncryptionContext := Structure.ActiveBranchKeyEncryptionContext(decryptOnlyEncryptionContext);
     var beaconEncryptionContext := Structure.BeaconKeyEncryptionContext(decryptOnlyEncryptionContext);
 
-    :- Need(KMSKeystoreOperations.AttemptKmsOperation?(kmsConfiguration, decryptOnlyEncryptionContext),
-            Types.KeyStoreException(message := "Invalid KMS Key ARN configured for GenerateDataKeyWithoutPlaintext in CreateBranchAndBeaconKeys."));
+    assert KMSKeystoreOperations.AttemptKmsOperation?(kmsConfiguration, decryptOnlyEncryptionContext);
     var wrappedDecryptOnlyBranchKey :- KMSKeystoreOperations.GenerateKey(
       decryptOnlyEncryptionContext,
       kmsConfiguration,
       grantTokens,
       kmsClient
     );
-    :- Need(KMSKeystoreOperations.AttemptKmsOperation?(kmsConfiguration, activeEncryptionContext),
-            Types.KeyStoreException(message := "Invalid KMS Key ARN configured for ReEncrypt in CreateBranchAndBeaconKeys."));
+    assert KMSKeystoreOperations.AttemptKmsOperation?(kmsConfiguration, activeEncryptionContext);
     var wrappedActiveBranchKey :- KMSKeystoreOperations.ReEncryptKey(
       wrappedDecryptOnlyBranchKey.CiphertextBlob.value,
       decryptOnlyEncryptionContext,
@@ -255,8 +253,7 @@ module {:options "/functionSyntax:4" } CreateKeys {
       grantTokens,
       kmsClient
     );
-    :- Need(KMSKeystoreOperations.AttemptKmsOperation?(kmsConfiguration, beaconEncryptionContext),
-            Types.KeyStoreException(message := "Invalid KMS Key ARN configured for GenerateDataKeyWithoutPlaintext(beacon key) in CreateBranchAndBeaconKeys."));
+    assert KMSKeystoreOperations.AttemptKmsOperation?(kmsConfiguration, beaconEncryptionContext);
     var wrappedBeaconKey :- KMSKeystoreOperations.GenerateKey(
       beaconEncryptionContext,
       kmsConfiguration,
@@ -264,26 +261,21 @@ module {:options "/functionSyntax:4" } CreateKeys {
       kmsClient
     );
 
-
-    var decryptOnlyBranchKeyItem := Structure.ToAttributeMap(
-      decryptOnlyEncryptionContext,
-      wrappedDecryptOnlyBranchKey.CiphertextBlob.value
-    );
-    var activeBranchKeyItem := Structure.ToAttributeMap(
-      activeEncryptionContext,
-      wrappedActiveBranchKey.CiphertextBlob.value
-    );
-    var beaconKeyItem := Structure.ToAttributeMap(
-      beaconEncryptionContext,
-      wrappedBeaconKey.CiphertextBlob.value
-    );
-
-    var _ :- DDBKeystoreOperations.WriteNewKeyToStore(
-      decryptOnlyBranchKeyItem,
-      activeBranchKeyItem,
-      beaconKeyItem,
-      ddbTableName,
-      ddbClient
+    var _ :- storage.WriteNewEncryptedBranchKey(
+      Types.WriteNewEncryptedBranchKeyInput(
+        Active := Structure.ConstructEncryptedHierarchicalKey(
+          activeEncryptionContext,
+          wrappedActiveBranchKey.CiphertextBlob.value
+        ),
+        Version := Structure.ConstructEncryptedHierarchicalKey(
+          decryptOnlyEncryptionContext,
+          wrappedDecryptOnlyBranchKey.CiphertextBlob.value
+        ),
+        Beacon := Structure.ConstructEncryptedHierarchicalKey(
+          beaconEncryptionContext,
+          wrappedBeaconKey.CiphertextBlob.value
+        )
+      )
     );
 
     output := Success(
@@ -296,101 +288,115 @@ module {:options "/functionSyntax:4" } CreateKeys {
     input: Types.VersionKeyInput,
     timestamp: string,
     branchKeyVersion: string,
-    ddbTableName: DDB.TableName,
     logicalKeyStoreName: string,
     kmsConfiguration: Types.KMSConfiguration,
     grantTokens: KMS.GrantTokenList,
     kmsClient: KMS.IKMSClient,
-    ddbClient: DDB.IDynamoDBClient
+    storage: Types.IKeyStorageInterface
   )
     returns (output: Result<Types.VersionKeyOutput, Types.Error>)
     requires 0 < |input.branchKeyIdentifier| && 0 < |branchKeyVersion|
-    requires ddbClient.Modifies !! kmsClient.Modifies
+    requires storage.Modifies !! kmsClient.Modifies
     requires KMSKeystoreOperations.HasKeyId(kmsConfiguration) && KmsArn.ValidKmsArn?(KMSKeystoreOperations.GetKeyId(kmsConfiguration))
+    requires storage is DefaultKeyStorageInterface.DynamoDBKeyStorageInterface
+             ==>
+               logicalKeyStoreName == (storage as DefaultKeyStorageInterface.DynamoDBKeyStorageInterface).logicalKeyStoreName
 
-    requires kmsClient.ValidState() && ddbClient.ValidState()
-    modifies ddbClient.Modifies, kmsClient.Modifies
-    ensures ddbClient.ValidState() && kmsClient.ValidState()
+    requires kmsClient.ValidState() && storage.ValidState()
+    modifies storage.Modifies, kmsClient.Modifies
+    ensures storage.ValidState() && kmsClient.ValidState()
+
+    //= aws-encryption-sdk-specification/framework/branch-key-store.md#versionkey
+    //= type=implication
+    //# VersionKey MUST first get the active version for the branch key from the keystore
+    //# by calling the configured [KeyStorage interface's](./key-store/key-storage.md#interface)
+    //# [GetEncryptedActiveBranchKey](./key-store/key-storage.md#getencryptedactivebranchkey)
+    //# using the `branch-key-id`.
+    ensures
+      && |storage.History.GetEncryptedActiveBranchKey| == |old(storage.History.GetEncryptedActiveBranchKey)| + 1
+      && Seq.Last(storage.History.GetEncryptedActiveBranchKey).input.Identifier == input.branchKeyIdentifier
 
     ensures output.Success?
             ==>
-              //= aws-encryption-sdk-specification/framework/branch-key-store.md#versionkey
-              //= type=implication
-              //# VersionKey MUST first get the active version for the branch key from the keystore
-              //# by calling AWS DDB `GetItem`
-              //# using the `branch-key-id` as the Partition Key and `"branch:ACTIVE"` value as the Sort Key.
-              && |ddbClient.History.GetItem| == |old(ddbClient.History.GetItem)| + 1
-              && Seq.Last(ddbClient.History.GetItem).input.Key
-                 == map[
-                      Structure.BRANCH_KEY_IDENTIFIER_FIELD := DDB.AttributeValue.S(input.branchKeyIdentifier),
-                      Structure.TYPE_FIELD := DDB.AttributeValue.S(Structure.BRANCH_KEY_ACTIVE_TYPE)
-                    ]
+              && Seq.Last(storage.History.GetEncryptedActiveBranchKey).output.Success?
+              && var oldActiveItem := Seq.Last(storage.History.GetEncryptedActiveBranchKey).output.value.Item;
 
-              && Seq.Last(ddbClient.History.GetItem).output.Success?
-              && Seq.Last(ddbClient.History.GetItem).output.value.Item.Some?
-              && var oldActiveItem := Seq.Last(ddbClient.History.GetItem).output.value.Item.value;
-              && Structure.BranchKeyItem?(oldActiveItem)
-              && Structure.BRANCH_KEY_ACTIVE_VERSION_FIELD in oldActiveItem
 
               //= aws-encryption-sdk-specification/framework/branch-key-store.md#versionkey
               //= type=implication
-              //# The `kms-arn` field of DDB response item MUST be [compatible with](#aws-key-arn-compatibility)
+              //# VersionKey MUST verify that the returned EncryptedHierarchicalKey MUST have the requested `branch-key-id`.
+              && oldActiveItem.Identifier == input.branchKeyIdentifier
+
+              //= aws-encryption-sdk-specification/framework/branch-key-store.md#versionkey
+              //= type=implication
+              //# VersionKey MUST verify that the returned EncryptedHierarchicalKey is an ActiveHierarchicalSymmetricVersion.
+              && Structure.ActiveHierarchicalSymmetricKey?(oldActiveItem)
+
+              //= aws-encryption-sdk-specification/framework/branch-key-store.md#versionkey
+              //= type=implication
+              //# VersionKey MUST verify that the returned EncryptedHierarchicalKey MUST have a logical table name equal to the configured logical table name.
+              && oldActiveItem.EncryptionContext[Structure.TABLE_FIELD] == logicalKeyStoreName
+
+              //= aws-encryption-sdk-specification/framework/branch-key-store.md#versionkey
+              //= type=implication
+              //# The `KmsArn` of the [EncryptedHierarchicalKey](./key-store/key-storage.md#encryptedhierarchicalkey)
+              //# MUST be [compatible with](#aws-key-arn-compatibility)
               //# the configured `KMS ARN` in the [AWS KMS Configuration](#aws-kms-configuration) for this keystore.
-              && KMSKeystoreOperations.AttemptKmsOperation?(kmsConfiguration, Structure.ToBranchKeyContext(oldActiveItem, logicalKeyStoreName))
-
-              && Structure.KMS_FIELD in oldActiveItem
-              && KMSKeystoreOperations.Compatible?(kmsConfiguration, oldActiveItem[Structure.KMS_FIELD].S)
+              && KMSKeystoreOperations.AttemptKmsOperation?(kmsConfiguration, oldActiveItem.EncryptionContext)
+              && KMSKeystoreOperations.Compatible?(kmsConfiguration, oldActiveItem.KmsArn)
 
               //= aws-encryption-sdk-specification/framework/branch-key-store.md#versionkey
               //= type=implication
-              //# The values on the AWS DDB response item
-              //# MUST be authenticated according to [authenticating a keystore item](#authenticating-a-keystore-item).
+              //# The [EncryptedHierarchicalKey](./key-store/key-storage.md#encryptedhierarchicalkey)
+              //# MUST be authenticated according to [authenticating a keystore item](#authenticating-an-encryptedhierarchicalkey).
 
-              //= aws-encryption-sdk-specification/framework/branch-key-store.md#authenticating-a-keystore-item
+              //= aws-encryption-sdk-specification/framework/branch-key-store.md#authenticating-an-encryptedhierarchicalkey
               //= type=implication
               //# The operation MUST use the configured `KMS SDK Client` to authenticate the value of the keystore item.
               && |kmsClient.History.ReEncrypt| == |old(kmsClient.History.ReEncrypt)| + 2 // This 2 because we need to wrap the new version
 
-              //= aws-encryption-sdk-specification/framework/branch-key-store.md#authenticating-a-keystore-item
+              //= aws-encryption-sdk-specification/framework/branch-key-store.md#authenticating-an-encryptedhierarchicalkey
               //= type=implication
               //# The operation MUST call [AWS KMS API ReEncrypt](https://docs.aws.amazon.com/kms/latest/APIReference/API_ReEncrypt.html)
               //# with a request constructed as follows:
               && var reEncryptInput := Seq.Last(Seq.DropLast(kmsClient.History.ReEncrypt)).input;
 
-              //= aws-encryption-sdk-specification/framework/branch-key-store.md#authenticating-a-keystore-item
+              //= aws-encryption-sdk-specification/framework/branch-key-store.md#authenticating-an-encryptedhierarchicalkey
               //= type=implication
-              //# - `SourceEncryptionContext` MUST be the [encryption context](#encryption-context) constructed above
-              && reEncryptInput.SourceEncryptionContext == Some(Structure.ToBranchKeyContext(oldActiveItem, logicalKeyStoreName))
+              //# - `SourceEncryptionContext` MUST be the [encryption context](#encryption-context) of the EncryptedHierarchicalKey to be authenticated
+              && reEncryptInput.SourceEncryptionContext == Some(oldActiveItem.EncryptionContext)
 
-              //= aws-encryption-sdk-specification/framework/branch-key-store.md#authenticating-a-keystore-item
+              //= aws-encryption-sdk-specification/framework/branch-key-store.md#authenticating-an-encryptedhierarchicalkey
               //= type=implication
               //# - `SourceKeyId` MUST be [compatible with](#aws-key-arn-compatibility) the configured KMS Key in the [AWS KMS Configuration](#aws-kms-configuration) for this keystore.
               && KMSKeystoreOperations.OptCompatible?(kmsConfiguration, reEncryptInput.SourceKeyId)
 
-              //= aws-encryption-sdk-specification/framework/branch-key-store.md#authenticating-a-keystore-item
+              //= aws-encryption-sdk-specification/framework/branch-key-store.md#authenticating-an-encryptedhierarchicalkey
               //= type=implication
-              //# - `CiphertextBlob` MUST be the `enc` attribute value on the AWS DDB response item
-              && reEncryptInput.CiphertextBlob == oldActiveItem[Structure.BRANCH_KEY_FIELD].B
+              //# - `CiphertextBlob` MUST be the `CiphertextBlob` attribute value on the EncryptedHierarchicalKey to be authenticated
+              && reEncryptInput.CiphertextBlob == oldActiveItem.CiphertextBlob
 
-              //= aws-encryption-sdk-specification/framework/branch-key-store.md#authenticating-a-keystore-item
+              //= aws-encryption-sdk-specification/framework/branch-key-store.md#authenticating-an-encryptedhierarchicalkey
               //= type=implication
               //# - `GrantTokens` MUST be the configured [grant tokens](https://docs.aws.amazon.com/kms/latest/developerguide/concepts.html#grant_token).
               && reEncryptInput.GrantTokens == Some(grantTokens)
 
-              //= aws-encryption-sdk-specification/framework/branch-key-store.md#authenticating-a-keystore-item
+              //= aws-encryption-sdk-specification/framework/branch-key-store.md#authenticating-an-encryptedhierarchicalkey
               //= type=implication
               //# - `DestinationKeyId` MUST be [compatible with](#aws-key-arn-compatibility) the configured KMS Key in the [AWS KMS Configuration](#aws-kms-configuration) for this keystore.
               && KMSKeystoreOperations.Compatible?(kmsConfiguration, reEncryptInput.DestinationKeyId)
 
-              //= aws-encryption-sdk-specification/framework/branch-key-store.md#authenticating-a-keystore-item
+              //= aws-encryption-sdk-specification/framework/branch-key-store.md#authenticating-an-encryptedhierarchicalkey
               //= type=implication
-              //# - `DestinationEncryptionContext` MUST be the [encryption context](#encryption-context) constructed above
-              && reEncryptInput.DestinationEncryptionContext == Some(Structure.ToBranchKeyContext(oldActiveItem, logicalKeyStoreName))
+              //# - `DestinationEncryptionContext` MUST be the [encryption context](#encryption-context) of the EncryptedHierarchicalKey to be authenticated
+              && reEncryptInput.DestinationEncryptionContext == Some(oldActiveItem.EncryptionContext)
 
               && |kmsClient.History.GenerateDataKeyWithoutPlaintext| == |old(kmsClient.History.GenerateDataKeyWithoutPlaintext)| + 1
+              && old(kmsClient.History.GenerateDataKeyWithoutPlaintext) < kmsClient.History.GenerateDataKeyWithoutPlaintext
+              && old(kmsClient.History.ReEncrypt) < kmsClient.History.ReEncrypt
 
               && var decryptOnlyEncryptionContext := Structure.NewVersionFromActiveBranchKeyEncryptionContext(
-                                                       Structure.ToBranchKeyContext(oldActiveItem, logicalKeyStoreName),
+                                                       oldActiveItem.EncryptionContext,
                                                        branchKeyVersion,
                                                        timestamp
                                                      );
@@ -407,50 +413,40 @@ module {:options "/functionSyntax:4" } CreateKeys {
                    decryptOnlyEncryptionContext
                  )
 
-              //= aws-encryption-sdk-specification/framework/branch-key-store.md#versionkey
-              //= type=implication
-              //# The call to Amazon DynamoDB TransactWriteItems MUST use the configured Amazon DynamoDB Client to make the call.
+              && |storage.History.WriteNewEncryptedBranchKeyVersion| == |old(storage.History.WriteNewEncryptedBranchKeyVersion)| + 1
 
               //= aws-encryption-sdk-specification/framework/branch-key-store.md#versionkey
               //= type=implication
-              //# To add the new branch key to the keystore,
-              //# the operation MUST call [Amazon DynamoDB API TransactWriteItems](https://docs.aws.amazon.com/amazondynamodb/latest/APIReference/API_TransactWriteItems.html).
-              && |ddbClient.History.TransactWriteItems| == |old(ddbClient.History.TransactWriteItems)| + 1
+              //# If creation of the keys are successful,
+              //# then the key store MUST call the configured [KeyStorage interface's](./key-store/key-storage.md#interface)
+              //# [WriteNewEncryptedBranchKeyVersion](./key-store/key-storage.md##writenewencryptedbranchkeyversion)
+              //# with these 2 [EncryptedHierarchicalKeys](./key-store/key-storage.md##encryptedhierarchicalkey).
+              && Seq.Last(storage.History.WriteNewEncryptedBranchKeyVersion).input.Active
+                 == Structure.ConstructEncryptedHierarchicalKey(
+                      Seq.Last(kmsClient.History.ReEncrypt).input.DestinationEncryptionContext.value,
+                      Seq.Last(kmsClient.History.ReEncrypt).output.value.CiphertextBlob.value
+                    )
+
+              && Seq.Last(storage.History.WriteNewEncryptedBranchKeyVersion).input.Version
+                 == Structure.ConstructEncryptedHierarchicalKey(
+                      Seq.Last(kmsClient.History.GenerateDataKeyWithoutPlaintext).input.EncryptionContext.value,
+                      Seq.Last(kmsClient.History.GenerateDataKeyWithoutPlaintext).output.value.CiphertextBlob.value
+                    )
 
               //= aws-encryption-sdk-specification/framework/branch-key-store.md#versionkey
               //= type=implication
-              //# The operation MUST call Amazon DynamoDB TransactWriteItems with a request constructed as follows:
-              && var writeNewKey := Seq.Last(ddbClient.History.TransactWriteItems).input;
+              //# The `kms-arn` stored in the table MUST NOT change as a result of this operation,
+              //# even if the KeyStore is configured with a `KMS MRKey ARN` that does not exactly match the stored ARN.
+              && Seq.Last(storage.History.WriteNewEncryptedBranchKeyVersion).input.Active.KmsArn == oldActiveItem.KmsArn
+              && Seq.Last(storage.History.WriteNewEncryptedBranchKeyVersion).input.Version.KmsArn == oldActiveItem.KmsArn
 
-              && 2 == |writeNewKey.TransactItems|
+              && Seq.Last(storage.History.WriteNewEncryptedBranchKeyVersion).output.Success?
 
-              && writeNewKey.TransactItems[0].Put.Some?
-              && writeNewKey.TransactItems[0].Put.value.Item
-                 == Structure.ToAttributeMap(
-                      decryptOnlyEncryptionContext,
-                      //= aws-encryption-sdk-specification/framework/branch-key-store.md#wrapped-branch-key-creation
-                      //= type=implication
-                      //# If the call to AWS KMS GenerateDataKeyWithoutPlaintext succeeds,
-                      //# the operation MUST use the GenerateDataKeyWithoutPlaintext result `CiphertextBlob`
-                      //# as the wrapped DECRYPT_ONLY Branch Key.
-                      Seq.Last(kmsClient.History.GenerateDataKeyWithoutPlaintext).output.value.CiphertextBlob.value)
-
-              && writeNewKey.TransactItems[1].Put.Some?
-              && writeNewKey.TransactItems[1].Put.value.Item
-                 == Structure.ToAttributeMap(
-                      Structure.ActiveBranchKeyEncryptionContext(decryptOnlyEncryptionContext),
-                      //= aws-encryption-sdk-specification/framework/branch-key-store.md#wrapped-branch-key-creation
-                      //= type=implication
-                      //# If the call to AWS KMS ReEncrypt succeeds,
-                      //# the operation MUST use the ReEncrypt result `CiphertextBlob`
-                      //# as the wrapped ACTIVE Branch Key.
-                      Seq.Last(kmsClient.History.ReEncrypt).output.value.CiphertextBlob.value)
-
-              && Seq.Last(ddbClient.History.TransactWriteItems).output.Success?
 
               //= aws-encryption-sdk-specification/framework/branch-key-store.md#versionkey
               //= type=implication
-              //# If DDB TransactWriteItems is successful, this operation MUST return a successful response containing no additional data.
+              //# If the [WriteNewEncryptedBranchKeyVersion](./key-store/key-storage.md#writenewencryptedbranchkeyversion) is successful,
+              //# this operation MUST return a successful response containing no additional data.
               && output == Success(Types.VersionKeyOutput)
 
     ensures
@@ -464,7 +460,6 @@ module {:options "/functionSyntax:4" } CreateKeys {
       //= aws-encryption-sdk-specification/framework/branch-key-store.md#versionkey
       //= type=implication
       //# Otherwise, this operation MUST yield an error.
-
       || (&& |kmsClient.History.GenerateDataKeyWithoutPlaintext| == |old(kmsClient.History.GenerateDataKeyWithoutPlaintext)| + 1
           && Seq.Last(kmsClient.History.GenerateDataKeyWithoutPlaintext).output.Failure?
           ==> output.Failure?)
@@ -473,37 +468,51 @@ module {:options "/functionSyntax:4" } CreateKeys {
           && Seq.Last(kmsClient.History.ReEncrypt).output.Failure?
           ==> output.Failure?)
 
-      || (&& |ddbClient.History.TransactWriteItems| == |old(ddbClient.History.TransactWriteItems)| + 1
-          && Seq.Last(ddbClient.History.TransactWriteItems).output.Failure?
+      || (&& |storage.History.GetEncryptedActiveBranchKey| == |old(storage.History.GetEncryptedActiveBranchKey)| + 1
+          && Seq.Last(storage.History.WriteNewEncryptedBranchKeyVersion).output.Failure?
+          ==> output.Failure?)
+
+      || (&& |storage.History.WriteNewEncryptedBranchKeyVersion| == |old(storage.History.WriteNewEncryptedBranchKeyVersion)| + 1
+          && Seq.Last(storage.History.WriteNewEncryptedBranchKeyVersion).output.Failure?
           ==> output.Failure?)
 
   {
 
-    var oldActiveItem :- DDBKeystoreOperations.GetActiveBranchKeyItem(
-      input.branchKeyIdentifier,
-      ddbTableName,
-      ddbClient
+    var GetEncryptedActiveBranchKeyOutput :- storage.GetEncryptedActiveBranchKey(
+      Types.GetEncryptedActiveBranchKeyInput(
+        Identifier := input.branchKeyIdentifier
+      )
     );
-
-    var oldActiveEncryptionContext := Structure.ToBranchKeyContext(oldActiveItem, logicalKeyStoreName);
+    var oldActiveItem := GetEncryptedActiveBranchKeyOutput.Item;
 
     :- Need(
-      && KMSKeystoreOperations.AttemptKmsOperation?(kmsConfiguration, oldActiveEncryptionContext),
+      || storage is DefaultKeyStorageInterface.DynamoDBKeyStorageInterface
+      || (
+           && oldActiveItem.Identifier == input.branchKeyIdentifier
+           && Structure.ActiveHierarchicalSymmetricKey?(oldActiveItem)
+           && oldActiveItem.EncryptionContext[Structure.TABLE_FIELD] == logicalKeyStoreName
+         ),
+      Types.KeyStoreException(
+        message := ErrorMessages.INVALID_ACTIVE_BRANCH_KEY_FROM_STORAGE)
+    );
+
+    :- Need(
+      && KMSKeystoreOperations.AttemptKmsOperation?(kmsConfiguration, oldActiveItem.EncryptionContext),
       Types.KeyStoreException(
         message := ErrorMessages.VERSION_KEY_KMS_KEY_ARN_DISAGREEMENT)
     );
 
     var _ :- KMSKeystoreOperations.ReEncryptKey(
-      oldActiveItem[Structure.BRANCH_KEY_FIELD].B,
-      oldActiveEncryptionContext,
-      oldActiveEncryptionContext,
+      oldActiveItem.CiphertextBlob,
+      oldActiveItem.EncryptionContext,
+      oldActiveItem.EncryptionContext,
       kmsConfiguration,
       grantTokens,
       kmsClient
     );
 
     var decryptOnlyEncryptionContext := Structure.NewVersionFromActiveBranchKeyEncryptionContext(
-      oldActiveEncryptionContext,
+      oldActiveItem.EncryptionContext,
       branchKeyVersion,
       timestamp
     );
@@ -527,34 +536,30 @@ module {:options "/functionSyntax:4" } CreateKeys {
       kmsClient
     );
 
-    var decryptOnlyBranchKeyItem: Structure.VersionBranchKeyItem := Structure.ToAttributeMap(
-      decryptOnlyEncryptionContext,
-      wrappedDecryptOnlyBranchKey.CiphertextBlob.value
+    var _ :- storage.WriteNewEncryptedBranchKeyVersion(
+      Types.WriteNewEncryptedBranchKeyVersionInput(
+        Active :=  Structure.ConstructEncryptedHierarchicalKey(
+          activeEncryptionContext,
+          wrappedActiveBranchKey.CiphertextBlob.value
+        ),
+        Version :=  Structure.ConstructEncryptedHierarchicalKey(
+          decryptOnlyEncryptionContext,
+          wrappedDecryptOnlyBranchKey.CiphertextBlob.value
+        ),
+        oldActive := oldActiveItem
+      )
     );
-    var activeBranchKeyItem: Structure.ActiveBranchKeyItem := Structure.ToAttributeMap(
-      activeEncryptionContext,
-      wrappedActiveBranchKey.CiphertextBlob.value
-    );
-
-    var _ :- DDBKeystoreOperations.WriteNewBranchKeyVersionToKeystore(
-      decryptOnlyBranchKeyItem,
-      activeBranchKeyItem,
-      ddbTableName,
-      ddbClient
-    );
-
-    assert && |ddbClient.History.TransactWriteItems| == |old(ddbClient.History.TransactWriteItems)| + 1;
 
     output := Success(Types.VersionKeyOutput());
   }
 
 
-  ghost predicate WrappedBranchKeyCreation?(
+  twostate predicate WrappedBranchKeyCreation?(
     //= aws-encryption-sdk-specification/framework/branch-key-store.md#wrapped-branch-key-creation
     //= type=implication
     //# The operation MUST call [AWS KMS API GenerateDataKeyWithoutPlaintext](https://docs.aws.amazon.com/kms/latest/APIReference/API_GenerateDataKeyWithoutPlaintext.html).
-    generateHistory: KMS.DafnyCallEvent<KMS.GenerateDataKeyWithoutPlaintextRequest, Result<KMS.GenerateDataKeyWithoutPlaintextResponse, KMS.Error>>,
-    reEncryptHistory: KMS.DafnyCallEvent<KMS.ReEncryptRequest, Result<KMS.ReEncryptResponse, KMS.Error>>,
+    new generateHistory: KMS.DafnyCallEvent<KMS.GenerateDataKeyWithoutPlaintextRequest, Result<KMS.GenerateDataKeyWithoutPlaintextResponse, KMS.Error>>,
+    new reEncryptHistory: KMS.DafnyCallEvent<KMS.ReEncryptRequest, Result<KMS.ReEncryptResponse, KMS.Error>>,
     kmsClient: KMS.IKMSClient,
     kmsConfiguration: Types.KMSConfiguration,
     grantTokens: KMS.GrantTokenList,
@@ -563,17 +568,17 @@ module {:options "/functionSyntax:4" } CreateKeys {
     reads kmsClient.History
     requires KMSKeystoreOperations.HasKeyId(kmsConfiguration) && KmsArn.ValidKmsArn?(KMSKeystoreOperations.GetKeyId(kmsConfiguration))
 
-    requires Structure.BranchKeyContext?(decryptOnlyEncryptionContext)
-    requires Structure.BRANCH_KEY_TYPE_PREFIX < decryptOnlyEncryptionContext[Structure.TYPE_FIELD]
 
-    // Ideally this be in "the things I added"
-    // But I don't know how to express that yet.
+    // The history elements are "the things I added"
+    requires old(kmsClient.History.GenerateDataKeyWithoutPlaintext) < kmsClient.History.GenerateDataKeyWithoutPlaintext
+    requires old(kmsClient.History.ReEncrypt) < kmsClient.History.ReEncrypt
 
     //= aws-encryption-sdk-specification/framework/branch-key-store.md#wrapped-branch-key-creation
     //= type=implication
     //# The call to AWS KMS GenerateDataKeyWithoutPlaintext MUST use the configured AWS KMS client to make the call.
-    requires generateHistory in kmsClient.History.GenerateDataKeyWithoutPlaintext
-    requires reEncryptHistory in kmsClient.History.ReEncrypt
+    requires
+      && generateHistory in kmsClient.History.GenerateDataKeyWithoutPlaintext[|old(kmsClient.History.GenerateDataKeyWithoutPlaintext)|..]
+      && reEncryptHistory in kmsClient.History.ReEncrypt[|old(kmsClient.History.ReEncrypt)|..]
   {
 
     //= aws-encryption-sdk-specification/framework/branch-key-store.md#wrapped-branch-key-creation
@@ -594,6 +599,7 @@ module {:options "/functionSyntax:4" } CreateKeys {
     //= aws-encryption-sdk-specification/framework/branch-key-store.md#wrapped-branch-key-creation
     //= type=implication
     //# - `EncryptionContext` MUST be the [DECRYPT_ONLY encryption context for branch keys](#decrypt_only-encryption-context).
+    && Structure.BranchKeyContext?(decryptOnlyEncryptionContext)
     && decryptOnlyKmsInput.EncryptionContext == Some(decryptOnlyEncryptionContext)
 
     //= aws-encryption-sdk-specification/framework/branch-key-store.md#wrapped-branch-key-creation
@@ -634,6 +640,9 @@ module {:options "/functionSyntax:4" } CreateKeys {
     //= type=implication
     //# - `SourceEncryptionContext` MUST be the [DECRYPT_ONLY encryption context for branch keys](#decrypt_only-encryption-context).
     && activeInput.SourceEncryptionContext == Some(decryptOnlyEncryptionContext)
+
+    && Structure.BRANCH_KEY_TYPE_PREFIX < decryptOnlyEncryptionContext[Structure.TYPE_FIELD]
+    && Structure.BRANCH_KEY_ACTIVE_VERSION_FIELD !in decryptOnlyEncryptionContext
 
     //= aws-encryption-sdk-specification/framework/branch-key-store.md#wrapped-branch-key-creation
     //= type=implication
